NuPrim.thy
@@ -236,11 +236,19 @@ lemma ParamTag: "\<^bold>p\<^bold>a\<^bold>r\<^bold>a\<^bold>m x" for x :: "'a" 
   For example, "@{prop "\<And>bit_width value. \<^bold>p\<^bold>a\<^bold>r\<^bold>a\<^bold>m bit_width \<Longrightarrow> \<^bold>p\<^bold>a\<^bold>r\<^bold>a\<^bold>m value \<Longrightarrow> P bit_wdith value"},
     the first parameter `?bit_width` will be specified first and then the "?value".\<close>
 
-definition Premise :: "bool \<Rightarrow> prop" ("\<^bold>p\<^bold>r\<^bold>e\<^bold>m\<^bold>i\<^bold>s\<^bold>e _" [10] 9) where "Premise \<equiv> Trueprop"
+definition Premise :: "bool \<Rightarrow> prop" ("\<^bold>p\<^bold>r\<^bold>e\<^bold>m\<^bold>i\<^bold>s\<^bold>e _" [10] 9) where [\<nu>def]:"Premise \<equiv> Trueprop"
   \<comment> \<open>A tag to hint automatic provers to try to prove this proof obligation\<close>
 lemma [simp]: "\<^bold>p\<^bold>r\<^bold>e\<^bold>m\<^bold>i\<^bold>s\<^bold>e P \<equiv> Trueprop P"  unfolding Premise_def .
 lemma Premise_I: "P \<Longrightarrow> \<^bold>p\<^bold>r\<^bold>e\<^bold>m\<^bold>i\<^bold>s\<^bold>e P" by simp
+lemma Premise_E: "\<^bold>p\<^bold>r\<^bold>e\<^bold>m\<^bold>i\<^bold>s\<^bold>e P \<Longrightarrow> P" by simp
 lemma Premise_Irew: "(P \<Longrightarrow> PROP C) \<equiv> (\<^bold>p\<^bold>r\<^bold>e\<^bold>m\<^bold>i\<^bold>s\<^bold>e P \<Longrightarrow> PROP C)" by simp
+
+attribute_setup intro_premise = \<open>
+  Scan.succeed (Thm.rule_attribute [] (fn _ => fn th => th COMP @{thm Premise_I}))
+\<close>
+attribute_setup elim_premise = \<open>
+  Scan.succeed (Thm.rule_attribute [] (fn _ => fn th => th COMP @{thm Premise_E}))
+\<close>
 
 subsection \<open>Register and its collection\<close>
 
@@ -335,7 +343,7 @@ notation Proc_CtxTy ("(2\<flower_L>\<medium_left_bracket> _/ \<flower_L>\<flower
 consts Proc_Ctx_NoRegisters :: ind ("\<^bold>n\<^bold>o \<^bold>r\<^bold>e\<^bold>g\<^bold>i\<^bold>s\<^bold>t\<^bold>e\<^bold>r\<^bold>s")
 consts Proc_Ctx_EmptyStack :: ind ("\<^bold>e\<^bold>m\<^bold>p\<^bold>t\<^bold>y \<^bold>s\<^bold>t\<^bold>a\<^bold>c\<^bold>k")
 translations "x \<flower> \<^bold>n\<^bold>o \<^bold>r\<^bold>e\<^bold>g\<^bold>i\<^bold>s\<^bold>t\<^bold>e\<^bold>r\<^bold>s" == "x \<flower> CONST Void"
-  "\<^bold>e\<^bold>m\<^bold>p\<^bold>t\<^bold>y \<^bold>s\<^bold>t\<^bold>a\<^bold>c\<^bold>k \<flower> x" <= "CONST End_of_Contextual_Stack s \<flower> x"
+  "\<^bold>e\<^bold>m\<^bold>p\<^bold>t\<^bold>y \<^bold>s\<^bold>t\<^bold>a\<^bold>c\<^bold>k" <= "CONST End_of_Contextual_Stack s"
 lemma [elim]: "c \<in> (X \<flower> G) \<Longrightarrow> (\<And>x g. c = Proc_Ctx x g \<Longrightarrow> x \<in> X \<Longrightarrow> g \<in> G \<Longrightarrow> C) \<Longrightarrow> C"
   unfolding Proc_CtxTy_def by (cases c) auto
 lemma [intro]: "x \<in> X \<Longrightarrow> g \<in> G \<Longrightarrow> Proc_Ctx x g \<in> (X \<flower> G)" unfolding Proc_CtxTy_def by auto
@@ -410,9 +418,10 @@ definition begin_proc_ctx :: " ('a::lrep) \<Rightarrow> ('a \<flower> void) stat
 definition end_proc_ctx :: " ('a::lrep) \<flower> ('b::register_collection) \<Rightarrow> 'a state"
   where "end_proc_ctx ctx = (case ctx of Proc_Ctx x y \<Rightarrow> StatOn x)"
 
-lemma nop: "\<^bold>p\<^bold>r\<^bold>o\<^bold>c nop \<blangle> T \<longmapsto> T \<brangle>" unfolding nop_def Procedure_def by auto
+lemma nop_\<nu>proc: "\<^bold>p\<^bold>r\<^bold>o\<^bold>c nop \<blangle> T \<longmapsto> T \<brangle>" unfolding nop_def Procedure_def by auto
 lemma call: "\<^bold>p\<^bold>r\<^bold>o\<^bold>c f \<blangle> U \<longmapsto> V \<brangle> \<Longrightarrow> \<^bold>p\<^bold>r\<^bold>o\<^bold>c call f \<blangle> U \<flower> W \<longmapsto> V \<flower> W \<brangle>"
   unfolding call_def Procedure_def by  (auto simp add: bind_def)
+lemma begin_proc_ctx: "\<^bold>p\<^bold>r\<^bold>o\<^bold>c begin_proc_ctx \<blangle> S \<longmapsto> S \<flower> Void \<brangle>" unfolding begin_proc_ctx_def \<nu>def by auto
 lemma end_proc_ctx: "\<^bold>p\<^bold>r\<^bold>o\<^bold>c end_proc_ctx \<blangle> T \<flower> R \<longmapsto> T \<brangle>" unfolding Procedure_def end_proc_ctx_def by auto
 lemma instr_comp: "\<^bold>p\<^bold>r\<^bold>o\<^bold>c f \<blangle> A \<longmapsto> B \<brangle> \<Longrightarrow> \<^bold>p\<^bold>r\<^bold>o\<^bold>c g \<blangle> B \<longmapsto> C \<brangle> \<Longrightarrow> \<^bold>p\<^bold>r\<^bold>o\<^bold>c (f \<nuInstrComp> g) \<blangle> A \<longmapsto> C \<brangle>"
   unfolding instr_comp_def Procedure_def bind_def by auto
@@ -583,26 +592,35 @@ lemma codeblock_export: "PROP Pure.prop (\<And>s. CodeBlock s a T f \<Longrighta
   qed
 qed
 
-theorem start_construction:
-  "CodeBlock s a S begin_proc_ctx \<Longrightarrow>
-      (\<^bold>c\<^bold>u\<^bold>r\<^bold>r\<^bold>e\<^bold>n\<^bold>t s \<^bold>r\<^bold>e\<^bold>s\<^bold>u\<^bold>l\<^bold>t\<^bold>s \<^bold>i\<^bold>n (S \<flower> Void) \<^bold>w\<^bold>i\<^bold>t\<^bold>h \<^bold>f\<^bold>a\<^bold>c\<^bold>t\<^bold>s: PROP FactCollection (PROP NoFact) (PROP NoFact) (PROP NoFact))"
-  for S :: " ('a::lrep) set" and a :: 'a and s :: "('a \<flower> void) state" including show_more1
-  unfolding begin_proc_ctx_def CodeBlock_def CurrentConstruction_def by (rule SpecTop_I; (rule FactCollection_I)?; (rule NoFact)?) auto
+lemma empty_facts: "PROP FactCollection (PROP NoFact) (PROP NoFact) (PROP NoFact)"
+  by ((rule FactCollection_I)?; (rule NoFact)?)
+theorem start_proc:
+  "CodeBlock s a S nop \<Longrightarrow> \<^bold>c\<^bold>u\<^bold>r\<^bold>r\<^bold>e\<^bold>n\<^bold>t s \<^bold>r\<^bold>e\<^bold>s\<^bold>u\<^bold>l\<^bold>t\<^bold>s \<^bold>i\<^bold>n S"
+  for S :: " ('a::lrep) set" and a :: 'a and s :: "'a state"
+  unfolding nop_def CodeBlock_def CurrentConstruction_def by auto
 
-theorem finish_construction: "(\<And>a s. CodeBlock s a S f \<Longrightarrow> (\<^bold>c\<^bold>u\<^bold>r\<^bold>r\<^bold>e\<^bold>n\<^bold>t s \<^bold>r\<^bold>e\<^bold>s\<^bold>u\<^bold>l\<^bold>t\<^bold>s \<^bold>i\<^bold>n (T \<flower> R)))
-  \<Longrightarrow> \<^bold>p\<^bold>r\<^bold>o\<^bold>c (f \<nuInstrComp> end_proc_ctx) \<blangle> S \<longmapsto> T \<brangle>" for S :: "('a::lrep) set" and  T :: "('b::lrep) set" and  R :: "('c::register_collection) set"
+theorem finish_proc: "(\<And>a s. CodeBlock s a S f \<Longrightarrow> (\<^bold>c\<^bold>u\<^bold>r\<^bold>r\<^bold>e\<^bold>n\<^bold>t s \<^bold>r\<^bold>e\<^bold>s\<^bold>u\<^bold>l\<^bold>t\<^bold>s \<^bold>i\<^bold>n T))
+  \<Longrightarrow> \<^bold>p\<^bold>r\<^bold>o\<^bold>c f \<blangle> S \<longmapsto> T \<brangle>" for S :: "('a::lrep) set" and  T :: "('b::lrep) set"
   unfolding CodeBlock_def Procedure_def
-proof
-  assume rule:"(\<And>a s. a \<in> S \<and> f a = s \<and> s \<noteq> SNeg \<Longrightarrow> (\<^bold>c\<^bold>u\<^bold>r\<^bold>r\<^bold>e\<^bold>n\<^bold>t s \<^bold>r\<^bold>e\<^bold>s\<^bold>u\<^bold>l\<^bold>t\<^bold>s \<^bold>i\<^bold>n (T \<flower> R)))"
-  fix a show "a \<in> S \<longrightarrow> (f \<nuInstrComp> end_proc_ctx) a \<in> \<S> T " proof
+  subgoal premises rule proof
+    fix a show "a \<in> S \<longrightarrow> f a \<in> \<S> T " proof
     assume a: "a \<in> S"
     moreover note rule[of a "f a", unfolded CurrentConstruction_def, simplified] 
-    ultimately show "(f \<nuInstrComp> end_proc_ctx) a \<in> \<S> T" unfolding instr_comp_def bind_def end_proc_ctx_def
+    ultimately show "f a \<in> \<S> T" unfolding instr_comp_def bind_def end_proc_ctx_def
       using LooseStateTy_introByStrict by (cases "f a") auto
-  qed
-qed
+  qed qed
+  done
 
-lemma rename_proc: "f \<equiv> f' \<Longrightarrow> \<^bold>p\<^bold>r\<^bold>o\<^bold>c f' \<blangle> U \<longmapsto> V \<brangle> \<Longrightarrow> \<^bold>p\<^bold>r\<^bold>o\<^bold>c f \<blangle> U \<longmapsto> V \<brangle>" by fast
+theorem start_block:
+  "((PROP X) \<^bold>w\<^bold>i\<^bold>t\<^bold>h \<^bold>f\<^bold>a\<^bold>c\<^bold>t\<^bold>s: PROP L) \<Longrightarrow>
+      CodeBlock s a U nop \<Longrightarrow>
+      (\<^bold>c\<^bold>u\<^bold>r\<^bold>r\<^bold>e\<^bold>n\<^bold>t s \<^bold>r\<^bold>e\<^bold>s\<^bold>u\<^bold>l\<^bold>t\<^bold>s \<^bold>i\<^bold>n U \<^bold>w\<^bold>i\<^bold>t\<^bold>h \<^bold>f\<^bold>a\<^bold>c\<^bold>t\<^bold>s: PROP L)"
+  for U :: " ('a::lrep) set" and V :: "('b::lrep) set" and s :: "'a state" and a :: 'a
+  unfolding nop_def CodeBlock_def CurrentConstruction_def SpecTop_imp by (rule SpecTop_I) auto
+
+lemma conj_imp: "(P \<and> Q \<Longrightarrow> PROP R) \<equiv> (P \<Longrightarrow> Q \<Longrightarrow> PROP R)" by rule simp+
+
+lemma rename_proc: "f \<equiv> f' \<Longrightarrow> \<^bold>p\<^bold>r\<^bold>o\<^bold>c f' \<blangle> U \<longmapsto> \<R> \<brangle> \<Longrightarrow> \<^bold>p\<^bold>r\<^bold>o\<^bold>c f \<blangle> U \<longmapsto> \<R> \<brangle>" by fast
 
 lemma name_star_fact:
   "\<^bold>p\<^bold>a\<^bold>r\<^bold>a\<^bold>m name \<Longrightarrow> (PROP P \<^bold>w\<^bold>i\<^bold>t\<^bold>h \<^bold>f\<^bold>a\<^bold>c\<^bold>t\<^bold>s: PROP FactCollection (Trueprop Q) (PROP L) (PROP S))
@@ -675,7 +693,6 @@ lemma [simp]: "T \<addition> True = T" unfolding AddtionTy_def by fast
 lemma [simp]: "\<S_S> (T \<addition> P) = (\<S_S> T \<addition> P)" unfolding AddtionTy_def by auto
 lemma [simp]: "((((\<^bold>c\<^bold>u\<^bold>r\<^bold>r\<^bold>e\<^bold>n\<^bold>t s \<^bold>r\<^bold>e\<^bold>s\<^bold>u\<^bold>l\<^bold>t\<^bold>s \<^bold>i\<^bold>n S) \<and> B) \<and> C) \<^bold>w\<^bold>i\<^bold>t\<^bold>h \<^bold>f\<^bold>a\<^bold>c\<^bold>t\<^bold>s: PROP L) \<equiv> (((\<^bold>c\<^bold>u\<^bold>r\<^bold>r\<^bold>e\<^bold>n\<^bold>t s \<^bold>r\<^bold>e\<^bold>s\<^bold>u\<^bold>l\<^bold>t\<^bold>s \<^bold>i\<^bold>n S) \<and> (B \<and> C)) \<^bold>w\<^bold>i\<^bold>t\<^bold>h \<^bold>f\<^bold>a\<^bold>c\<^bold>t\<^bold>s: PROP L)" by simp
 
-lemma conj_imp: "(P \<and> Q \<Longrightarrow> PROP R) \<equiv> (P \<Longrightarrow> Q \<Longrightarrow> PROP R)" by rule simp+
 lemma t1: "(\<^bold>c\<^bold>u\<^bold>r\<^bold>r\<^bold>e\<^bold>n\<^bold>t s \<^bold>r\<^bold>e\<^bold>s\<^bold>u\<^bold>l\<^bold>t\<^bold>s \<^bold>i\<^bold>n T \<addition> P) \<longleftrightarrow> (\<^bold>c\<^bold>u\<^bold>r\<^bold>r\<^bold>e\<^bold>n\<^bold>t s \<^bold>r\<^bold>e\<^bold>s\<^bold>u\<^bold>l\<^bold>t\<^bold>s \<^bold>i\<^bold>n T) \<and> P" unfolding CurrentConstruction_def AddtionTy_def by (cases s) auto
 lemma [simp]:
   "((\<^bold>c\<^bold>u\<^bold>r\<^bold>r\<^bold>e\<^bold>n\<^bold>t s \<^bold>r\<^bold>e\<^bold>s\<^bold>u\<^bold>l\<^bold>t\<^bold>s \<^bold>i\<^bold>n S \<addition> Q) \<^bold>w\<^bold>i\<^bold>t\<^bold>h \<^bold>f\<^bold>a\<^bold>c\<^bold>t\<^bold>s: PROP FactCollection (PROP NoFact) (PROP L) (PROP I))
@@ -730,10 +747,13 @@ theorem apply_proc_conv: "(\<^bold>c\<^bold>u\<^bold>r\<^bold>r\<^bold>e\<^bold>
   unfolding Procedure_def CurrentConstruction_def PendingConstruction_def bind_def SpecTop_imp Conversion_def by auto
 
 definition Atomic :: "'a \<Rightarrow> 'a" ("\<^bold>a\<^bold>t\<^bold>o\<^bold>m\<^bold>i\<^bold>c _" [501] 500) where "\<^bold>a\<^bold>t\<^bold>o\<^bold>m\<^bold>i\<^bold>c x = x"
-lemma [\<nu>auto_construct]: "\<^bold>p\<^bold>r\<^bold>o\<^bold>c nop \<blangle> t \<tycolon>T\<boxbar>Z \<longmapsto> \<^bold>a\<^bold>t\<^bold>o\<^bold>m\<^bold>i\<^bold>c t \<tycolon> T\<boxbar>Z \<brangle>" unfolding Atomic_def AutoTag_def using nop .
-lemma [\<nu>auto_destruct]: "\<^bold>p\<^bold>r\<^bold>o\<^bold>c nop \<blangle> t \<tycolon> \<^bold>a\<^bold>t\<^bold>o\<^bold>m\<^bold>i\<^bold>c T\<boxbar>Z \<longmapsto> t \<tycolon>T\<boxbar>Z \<brangle>" unfolding Atomic_def AutoTag_def using nop .
+lemma [\<nu>auto_construct]: "\<^bold>p\<^bold>r\<^bold>o\<^bold>c nop \<blangle> t \<tycolon>T\<boxbar>Z \<longmapsto> \<^bold>a\<^bold>t\<^bold>o\<^bold>m\<^bold>i\<^bold>c t \<tycolon> T\<boxbar>Z \<brangle>" unfolding Atomic_def AutoTag_def using nop_\<nu>proc .
+lemma [\<nu>auto_destruct]: "\<^bold>p\<^bold>r\<^bold>o\<^bold>c nop \<blangle> t \<tycolon> \<^bold>a\<^bold>t\<^bold>o\<^bold>m\<^bold>i\<^bold>c T\<boxbar>Z \<longmapsto> t \<tycolon>T\<boxbar>Z \<brangle>" unfolding Atomic_def AutoTag_def using nop_\<nu>proc .
 
-  section \<open>Finalize the syntax sugars to be ready for use\<close>
+  section \<open>Appendix\<close>
+
+subsection \<open>Finalize the syntax sugars to be ready for use\<close>
+
 no_translations "_pretty_and_ P Q" <= "CONST AndFact P Q"
 translations "_linebreak_collection_ P Q" <= "CONST AndFact P Q"
 
