NuBasicAbstractors.thy
@@ -1,9 +1,5 @@
 theory NuBasicAbstractors
   imports NuLLReps NuSys
-  abbrevs "SState" = "\<B_S>\<B_t>\<B_r>\<B_i>\<B_c>\<B_t>\<B_S>\<B_t>\<B_a>\<B_t>\<B_e>"
-      and "LState" = "\<B_L>\<B_o>\<B_o>\<B_s>\<B_e>\<B_S>\<B_t>\<B_a>\<B_t>\<B_e>" 
-      and "with_registers" = "\<B_w>\<B_i>\<B_t>\<B_h>_\<B_r>\<B_e>\<B_g>\<B_i>\<B_s>\<B_t>\<B_e>\<B_r>\<B_s>"
-      and "wreg" = "\<B_w>\<B_i>\<B_t>\<B_h>_\<B_r>\<B_e>\<B_g>\<B_i>\<B_s>\<B_t>\<B_e>\<B_r>\<B_s>"
 begin
 
 definition Fusion :: "('a1::lrep,'b1) nu \<Rightarrow> ('a2::lrep,'b2) nu \<Rightarrow> ('a1 \<times> 'a2, 'b1 \<times> 'b2) nu" (infixr "\<nuFusion>" 70) 
